add

UnitProJ/expressOS/Fall2015/INode-indexOf.dfy
@@ -57,6 +57,19 @@ spine == [this] + next.spine
 && next.ValidLemma())
 }
 
+predicate validSeqContentsLemma()
+	requires Valid();
+	reads this, footprint;
+	ensures validSeqContentsLemma();
+	ensures validSeqCond(spine);
+	ensures |tailContents| == |footprint|-1 == |spine|-1;
+  ensures forall i :: 0 <= i < |spine| ==> spine[i].data == ([data] + tailContents)[i];
+	ensures forall i :: 0 <= i < |spine| ==> spine[i].tailContents ==  ([data] + tailContents)[i+1..];
+{
+	ndValid2ListValidLemma() &&
+		next != null ==> next.validSeqContentsLemma()
+}
+
 method contains(tarNd:INode) returns (isIn:bool)
 	requires tarNd != null;
 	requires Valid();
@@ -118,6 +131,142 @@ assert tarNd !in footprint;
 return -1;
 }
 
+/////////////////////////////////////////
+
+method delete(pos:int) returns (delNd:INode)
+requires Valid();
+requires 0 < pos <= |tailContents|;
+
+modifies footprint;
+
+ensures Valid();
+ensures [data] + tailContents == old(([data] + tailContents)[0..pos] + ([data] + tailContents)[pos+1..] );
+ensures footprint == old(footprint) - {delNd};
+
+{
+var curNd := this;
+var curIndex := 0;
+
+assert ValidLemma();
+assert ndValid2ListValidLemma();
+assert validSeqContentsLemma();
+assert validSeqTCLemma(spine);
+
+while (curIndex < pos-1)
+invariant 0 <= curIndex < pos;
+invariant curNd != null && curNd.Valid();
+invariant validSeqCond(spine);
+invariant |curNd.tailContents| + curIndex == |tailContents|;
+invariant curNd.next != null;
+invariant curNd == spine[curIndex];
+
+invariant  spine[curIndex].data == ([data] + tailContents)[curIndex];
+
+invariant curNd.next == spine[curIndex+1];
+invariant curNd.next.next != null ==> curNd.next.next == spine[curIndex+2];
+
+modifies {};
+{
+curNd := curNd.next;
+curIndex := curIndex + 1;
+}
+
+delNd := curNd.next;
+
+delNext(curNd, delNd, pos);
+
+
+if(1 < pos <= |tailContents|) {
+ghost var oldContents := old([data] + tailContents); 
+ghost var newSpine := spine[0..pos-1];
+
+assert delNd != null;
+
+updateSeq4Del(newSpine, delNd, pos, curNd, oldContents, this);
+
+} else {}
+
+}
+
+////////////////////////////////////////////////////////
+method delNext(curNd: INode, delNd:INode, pos:int)
+  requires curNd != null && curNd.Valid();
+  requires curNd.next == delNd && delNd != null && delNd.Valid();
+	requires Valid();
+  requires 0 < pos < |spine| && spine[pos-1] == curNd;
+  requires validSeqCond(spine);
+
+	requires forall i :: 0 <= i <= pos-2 ==>
+	(|spine[i].tailContents|) >= pos - i;
+	requires |tailContents| >= pos;
+
+	requires curNd.data == ([data] + tailContents)[pos-1];
+	requires curNd.tailContents == ([data] + tailContents)[pos..];
+
+	requires |tailContents| == |spine|-1;
+	requires forall i :: 0 <= i <= pos-2 ==> spine[i].data == ([data] + tailContents)[i];
+
+//new
+requires	 (forall nd :: nd in spine ==> nd in footprint);
+	modifies curNd;
+	
+	ensures curNd.Valid();
+	ensures curNd.data == old(curNd.data) && curNd.next == delNd.next;
+	ensures curNd.footprint == old(curNd.footprint) - {delNd};
+	ensures curNd.tailContents == old(curNd.tailContents[1..]);
+	ensures curNd.spine == old([curNd.spine[0]] + curNd.spine[2..]);
+
+	ensures forall i :: 0 <= i <= pos-2 ==> spine[i].data == old(spine[i].data) &&
+		spine[i].next == old(spine[i].next) &&
+		spine[i].tailContents == old(spine[i].tailContents) &&
+		spine[i].footprint == old(spine[i].footprint) &&
+		spine[i].spine == old(spine[i].spine);
+
+		ensures listInv(spine[0..pos]);
+		ensures listCond(spine[0..pos-1]); 
+
+
+		ensures pos > 1 ==> spine[pos-2].tailContents == [curNd.data] + [delNd.data] + curNd.tailContents;
+
+		//new
+		ensures pos > 1 ==> spine[pos-2].footprint == {spine[pos-2]} + curNd.footprint + {delNd};
+
+	ensures forall i :: 0 <= i <= pos-2 ==>
+		(|spine[i].tailContents|) >= pos - i;
+
+		//	ensures pos > 1 ==>  footprint == old(footprint) && (set nd | nd in spine) <= old(footprint);
+
+		ensures pos > 1 ==>  footprint == old(footprint) &&
+		spine == old(spine) && (forall nd :: nd in spine ==> nd in footprint);
+		
+	//end new
+		
+		ensures forall i :: 0 <= i <= pos-2 ==>
+			(|spine[i].tailContents|) >= pos - i;
+
+			ensures	curNd.tailContents == old([data] + tailContents)[pos+1..];
+			
+			ensures forall i :: 0 <= i <= pos-2 ==> spine[i].data == old([data] + tailContents)[i];
+
+{
+	
+	curNd.next := curNd.next.next;
+
+if (curNd.next == null)
+{
+	curNd.tailContents := [];
+	curNd.footprint := {curNd};
+	curNd.spine := [curNd];
+}
+
+else {
+	curNd.tailContents := [curNd.next.data] + curNd.next.tailContents;
+	curNd.footprint := {curNd} + curNd.next.footprint;
+	curNd.spine := [curNd] + curNd.next.spine;
+}
+}
+////////////////////////////////////////
+
 
 predicate ndValid2ListValidLemma()
 requires Valid();
@@ -152,7 +301,10 @@ predicate spineTCLemma()
 	else spine == [this] + next.spine && tailContents == [next.data] + next.tailContents
 		&& next.spineTCLemma()
 }
+
 ////////////////////////////////////////////////////////
+//END of CLASS
+}
 
 function getFtprint(nd:INode): set<INode>
 reads nd;
@@ -168,6 +320,112 @@ ensures forall nd :: nd in mySeq ==>
 if mySeq == [] then {} else getFtprint(mySeq[0]) + sumAllFtprint(mySeq[1..])
 }
 
+ghost method updateSeq4Del(newSpine: seq<INode>, delNd:INode, pos: int, nxtNd:INode, oldContents:seq<Data>, thisNd:INode)
+	requires listCond(newSpine);
+	requires 1 < pos < |oldContents|;
+requires |newSpine| == pos - 1;
+
+requires nxtNd != null && nxtNd.Valid();
+requires newSpine[|newSpine|-1].next == nxtNd;
+
+//new
+requires thisNd == newSpine[0];
+
+requires delNd !in nxtNd.footprint && delNd !in newSpine;
+
+requires (set nd | nd in newSpine) !! nxtNd.footprint;
+requires newSpine[|newSpine|-1].footprint >= nxtNd.footprint;
+requires delNd != null;
+requires newSpine[|newSpine|-1].tailContents == [nxtNd.data] + [delNd.data] + nxtNd.tailContents;
+
+requires |newSpine[|newSpine|-1].tailContents| >= 2;
+
+requires newSpine[|newSpine|-1].footprint == {newSpine[|newSpine|-1]} + nxtNd.footprint + {delNd};
+	 
+requires  forall i :: 0 <= i <= pos-2 ==> (|newSpine[i].tailContents|) >= pos - i;
+
+requires |oldContents| > pos;
+requires nxtNd.tailContents == oldContents[pos+1..];
+requires nxtNd.data == oldContents[pos-1];
+requires forall i :: 0 <= i <= pos-2 ==> newSpine[i].data == oldContents[i];
+modifies newSpine;
+
+ensures thisNd.Valid();
+ensures  [thisNd.data] + thisNd.tailContents == oldContents[0..pos] + oldContents[pos+1..];
+
+ensures thisNd.footprint == old(thisNd.footprint) - {delNd};
+{
+
+ghost var curIndex := pos - 2;
+
+/////////pre to LI ok
+
+while(curIndex >= 0)
+
+	invariant -1 <= curIndex <= pos-2;
+
+	invariant newSpine[|newSpine|-1].next == nxtNd;
+
+	invariant nxtNd.Valid();
+
+  invariant newSpine == old(newSpine);
+	invariant thisNd == newSpine[0];
+
+	invariant listInv(newSpine);
+
+
+	invariant forall i :: 0 <= i <= curIndex ==> newSpine[i].tailContents == old(newSpine[i].tailContents) &&
+		newSpine[i].footprint == old(newSpine[i].footprint) && newSpine[i].spine == old(newSpine[i].spine);
+
+		//new
+		invariant forall i :: 0 <= i < curIndex ==> newSpine[i].footprint == {newSpine[i]} + newSpine[i+1].footprint
+			&&
+			newSpine[i].tailContents == [newSpine[i+1].data] + newSpine[i+1].tailContents;
+			
+		invariant -1 <= curIndex < pos-2 ==> newSpine[curIndex+1].footprint == old(newSpine[curIndex+1].footprint - {delNd});
+		
+invariant forall nd :: nd in newSpine ==> nd.data == old(nd.data);
+invariant nxtNd.data == old(nxtNd.data) && nxtNd.tailContents == old(nxtNd.tailContents);
+invariant oldContents == old(oldContents);
+
+invariant 0 <= curIndex <= pos-2 ==>  |newSpine[curIndex].tailContents| >= pos - curIndex;
+
+//new
+invariant -1 <= curIndex < pos - 2 ==>  [newSpine[curIndex+1].data] + newSpine[curIndex+1].tailContents == oldContents[curIndex+1..pos] + oldContents[pos+1..];	 
+//end new
+		
+ invariant -1 <= curIndex < pos - 2 ==> newSpine[curIndex+1].Valid();
+		
+	modifies newSpine;
+{
+newSpine[curIndex].tailContents :=  [newSpine[curIndex].next.data] + newSpine[curIndex].next.tailContents;
+newSpine[curIndex].footprint :=  {newSpine[curIndex]} + newSpine[curIndex].next.footprint;
+newSpine[curIndex].spine :=  [newSpine[curIndex]] + newSpine[curIndex].next.spine;
+
+curIndex := curIndex - 1;
+}
+
+assert curIndex == -1;
+
+assert newSpine[curIndex+1].Valid();
+
+assert [newSpine[curIndex+1].data] + newSpine[curIndex+1].tailContents == oldContents[curIndex+1..pos] + oldContents[pos+1..];
+
+assert newSpine[curIndex+1].footprint == old(newSpine[curIndex+1].footprint - {delNd});
+
+}
+
+predicate validSeqTCLemma(mySeq: seq<INode>)
+	requires validSeqCond(mySeq);
+	reads mySeq, (set nd | nd in mySeq);
+
+	ensures validSeqTCLemma(mySeq);
+	ensures forall i :: 0 <= i < |mySeq| ==> |mySeq[i].tailContents| == |mySeq| - 1 - i;
+{
+if |mySeq| <= 1 then true
+	else mySeq[0].tailContents == [mySeq[1].data] + mySeq[1].tailContents
+		&& validSeqTCLemma(mySeq[1..])
+}
 ///////////////////////////////////////////
 
 predicate listInv(mySeq: seq<INode>)
@@ -192,7 +450,6 @@ null !in mySeq && (forall nd :: nd in mySeq ==> nd in nd.footprint) &&
 && (forall i :: 0 <= i < |mySeq| ==> |mySeq|-i-1 <= |mySeq[i].tailContents|)
 }
 
-
 predicate validSeqCond(mySeq: seq<INode>)
 reads mySeq, (set nd | nd in mySeq);
 {
@@ -203,8 +460,6 @@ listCond(mySeq)
 && mySeq[|mySeq|-1].spine == [mySeq[|mySeq|-1]])
 }
 
-
-}
 
 //The INodes class: a list
 class INodes {
@@ -236,10 +491,10 @@ this in footprint
 //////////////////////////////////
 method contains(tarNd:INode) returns (isIn:bool)
 	requires valid();
-	requires tarNd != null;
+	requires tarNd != null && tarNd != head;
 	modifies {};
 	ensures valid();
-	ensures isIn <==> tarNd in head.footprint;
+	ensures isIn <==> tarNd in head.footprint - {head};
 {
 isIn := head.contains(tarNd);
 }
@@ -261,7 +516,16 @@ method indexOf(tarNd:INode) returns (index:int)
 	index := index - 1;
 }
 
-
-
+//del the given tarNd from the list
+/*
+method delNd(tarNd:INode)
+	requires valid();
+	requires tarNd != null;
+	modifies footprint;
+	ensures valid();
+	ensures tarNd !in footprint;
+	ensures 
+{}
+ */
 
 }
